$$
\begin{array}{ll}
-5 x+15 y-5 z=-20 & \text { (1) multiplied by }-5 \\
5 x-13 y+13 z=8 & \text { (3) } \\
2 y+8 z=-12
\end{array}
$$
Then, we multiply equation (4) by 2 and add it to equation (5).
$$
\begin{array}{l}
-2 y-8 z=14(4) \text { multiplied by } 2 \\
2 y+8 z=-12(5) \\
0=2
\end{array}
$$
The final equation $0=2$ is a contradiction, so we conclude that the system of equations in inconsistent and, therefore, has no solution.
(9) Analysis
In this system, each plane intersects the other two, but not at the same location. Therefore, the system is inconsistent.
TRY IT \#2 Solve the system of three equations in three variables.
$$
\begin{array}{c}
x+y+z=2 \\
y-3 z=1 \\
2 x+y+5 z=0
\end{array}
$$
Expressing the Solution of a System of Dependent Equations Containing Three Variables
We know from working with systems of equations in two variables that a dependent system of equations has an infinite number of solutions. The same is true for dependent systems of equations in three variables. An infinite number of solutions can result from several situations. The three planes could be the same, so that a solution to one equation will be the solution to the other two equations. All three equations could be different but they intersect on a line, which has infinite solutions. Or two of the equations could be the same and intersect the third on a line.
EXAMPLE 5
Finding the Solution to a Dependent System of Equations
Find the solution to the given system of three equations in three variables.
$$
\begin{array}{r}
2 x+y-3 z=0 \\
4 x+2 y-6 z=0 \\
x-y+z=0
\end{array}
$$
Solution
First, we can multiply equation (1) by -2 and add it to equation (2).
$$
\begin{array}{l}
-4 x-2 y+6 z=0 \text { equation(1) multiplied by }-2 \\
4 x+2 y-6 z=0 \quad \text { (2) } \\
0=0
\end{array}
$$
We do not need to proceed any further. The result we get is an identity, $0=0$, which tells us that this system has an infinite number of solutions. There are other ways to begin to solve this system, such as multiplying equation (3) by -2 , and adding it to equation (1). We then perform the same steps as above and find the same result, $0=0$.

When a system is dependent, we can find general expressions for the solutions. Adding equations (1) and (3), we have
$$
\begin{array}{c}
2 x+y-3 z=0 \\
x-y+z=0 \\
\hline 3 x-2 z=0
\end{array}
$$