V EXAMPLE I Given the graph of $y=\sqrt{x}$, use transformations to graph $y=\sqrt{x}-2$, $y=\sqrt{x-2}, y=-\sqrt{x}, y=2 \sqrt{x}$, and $y=\sqrt{-x}$.

SoLUtiOn The graph of the square root function $y=\sqrt{x}$, obtained from Figure 13(a) in Section 1.2, is shown in Figure 4(a). In the other parts of the figure we sketch $y=\sqrt{x}-2$ by shifting 2 units downward, $y=\sqrt{x-2}$ by shifting 2 units to the right, $y=-\sqrt{x}$ by reflecting about the $x$-axis, $y=2 \sqrt{x}$ by stretching vertically by a factor of 2 , and $y=\sqrt{-x}$ by reflecting about the $y$-axis.

![](https://cdn.mathpix.com/cropped/2023_03_05_049f094d450b314cf928g-1.jpg?height=317&width=230&top_left_y=564&top_left_x=126)

(a) $y=\sqrt{x}$

![](https://cdn.mathpix.com/cropped/2023_03_05_049f094d450b314cf928g-1.jpg?height=317&width=307&top_left_y=564&top_left_x=391)

(b) $y=\sqrt{x}-2$

![](https://cdn.mathpix.com/cropped/2023_03_05_049f094d450b314cf928g-1.jpg?height=317&width=301&top_left_y=564&top_left_x=729)

(c) $y=\sqrt{x-2}$

![](https://cdn.mathpix.com/cropped/2023_03_05_049f094d450b314cf928g-1.jpg?height=317&width=233&top_left_y=564&top_left_x=1067)

(d) $y=-\sqrt{x}$

![](https://cdn.mathpix.com/cropped/2023_03_05_049f094d450b314cf928g-1.jpg?height=317&width=238&top_left_y=564&top_left_x=1337)

(e) $y=2 \sqrt{x}$

![](https://cdn.mathpix.com/cropped/2023_03_05_049f094d450b314cf928g-1.jpg?height=317&width=238&top_left_y=564&top_left_x=1607)

(f) $y=\sqrt{-x}$

FIGURE 4

EXAMPLE 2 Sketch the graph of the function $f(x)=x^{2}+6 x+10$.

sOLUtion Completing the square, we write the equation of the graph as

$$
y=x^{2}+6 x+10=(x+3)^{2}+1
$$

This means we obtain the desired graph by starting with the parabola $y=x^{2}$ and shifting 3 units to the left and then 1 unit upward (see Figure 5).

![](https://cdn.mathpix.com/cropped/2023_03_05_049f094d450b314cf928g-1.jpg?height=359&width=442&top_left_y=1292&top_left_x=795)

FIGURE 5

![](https://cdn.mathpix.com/cropped/2023_03_05_049f094d450b314cf928g-1.jpg?height=353&width=419&top_left_y=1295&top_left_x=1317)

(b) $y=(x+3)^{2}+1$

EXAMPLE 3 Sketch the graphs of the following functions.
(a) $y=\sin (2 x)$
(b) $y=1-\sin (x)$

SOLUTION

(a) We obtain the graph of $y=\sin (2 x)$ from that of $y=\sin (x)$ by compressing horizontally by a factor of 2 (see Figures 6 and 7). Thus, whereas the period of $y=\sin (x)$ is $2 \pi$, the period of $y=\sin (2 x)$ is $2 \pi / 2=\pi$.

![](https://cdn.mathpix.com/cropped/2023_03_05_049f094d450b314cf928g-1.jpg?height=312&width=841&top_left_y=2007&top_left_x=124)

FIGURE 6

![](https://cdn.mathpix.com/cropped/2023_03_05_049f094d450b314cf928g-1.jpg?height=312&width=736&top_left_y=2007&top_left_x=1109)

FIGURE 7